use Fin N instead of RM

twophase/Twophase/Functional.lean
@@ -11,20 +11,14 @@ applicable to a given state, we return `none`.
 Compare it with the
 [TLA+ specification](https://github.com/tlaplus/Examples/blob/master/specifications/transaction_commit/TwoPhase.tla).
 
+Copyright (c) 2025 Igor Konnov
+Released under MIT license as described in the file LICENSE.
 Authors: Igor Konnov, 2025
 -/
 import Std.Data.HashMap
 import Mathlib.Data.Finset.Basic
-
--- The abstract type of resource managers.
-variable (RM : Type) [DecidableEq RM] [Hashable RM] [Repr RM]
-
-/-- A message that sent by either the transaction manager or a resource manager. -/
-inductive Message where
-    | Commit
-    | Abort
-    | Prepared(rm: RM)
-    deriving DecidableEq, Repr
+import Mathlib.Data.Finset.Range
+import Mathlib.Data.Finset.Fin
 
 /-- A state of a resource manager. -/
 inductive RMState where
@@ -41,23 +35,42 @@ inductive TMState where
     | Aborted
     deriving DecidableEq, Repr
 
+/-- A message that sent by either the transaction manager or a resource manager. -/
+inductive Message (N: Nat) where
+    | Commit
+    | Abort
+    | Prepared(i: Fin N)
+    deriving DecidableEq, Repr
+
 /-- A state of the Two-phase commit protocol. -/
-structure ProtocolState where
+structure ProtocolState (N: Nat) where
     -- The set of the resource managers.
     -- It may differ from run to run, but remains constant during a run.
-    all: Finset RM
-    rmState: Std.HashMap RM RMState
+    rmState: Std.HashMap (Fin N) RMState
     tmState: TMState
-    tmPrepared: Finset RM
-    msgs: Finset (Message RM)
+    tmPrepared: Finset (Fin N)
+    msgs: Finset (Message N)
 
 -- Functional behavior of the protocol
 section defs
+-- The number of resource managers.
+variable { N: Nat }
+-- A resource manager is represented by a number from 0 to N-1.
+abbrev RM (N: Nat) := Fin N
 -- The state `s` is a state of the protocol, explicitly added to all the functions.
-variable (s: ProtocolState RM)
+variable (s: ProtocolState N)
+
+-- We need this little theorem to construct the set of all resource managers.
+-- Fortunately, Lean can prove it itself.
+theorem mem_range_le: ∀ x ∈ Finset.range N, x < N := by
+    simp
+
+/-- The set of all resource managers. -/
+def AllRM: Finset (RM N) :=
+    Finset.attachFin (Finset.range N) mem_range_le
 
 /-- The transaction manager receives a `Prepared` message from a resource manager `rm`. -/
-def tmRcvPrepared (rm: RM) :=
+def tmRcvPrepared (rm: RM N) :=
     if s.tmState = TMState.Init ∧ Message.Prepared rm ∈ s.msgs then some {
         s with tmPrepared := s.tmPrepared ∪ { rm },
     } else none
@@ -67,7 +80,7 @@ def tmRcvPrepared (rm: RM) :=
   state and every RM has sent a `Prepared` message.
  -/
 def tmCommit :=
-    if s.tmState = TMState.Init ∧ s.tmPrepared = s.all then some {
+    if s.tmState = TMState.Init ∧ s.tmPrepared = AllRM then some {
         s with
         tmState := TMState.Committed,
         msgs := s.msgs ∪ { Message.Commit }
@@ -82,7 +95,7 @@ def tmAbort :=
     } else none
 
 /-- Resource manager `rm` prepares. -/
-def rmPrepare (rm: RM) :=
+def rmPrepare (rm: RM N) :=
     if s.rmState.get? rm = RMState.Working then some {
         s with
         rmState := s.rmState.insert rm RMState.Prepared,
@@ -91,19 +104,19 @@ def rmPrepare (rm: RM) :=
 
 /-- Resource manager $rm$ spontaneously decides to abort.  As noted above, `rm`
 does not send any message in our simplified spec. -/
-def rmChooseToAbort (rm: RM) :=
+def rmChooseToAbort (rm: RM N) :=
     if s.rmState.get? rm = RMState.Working then some {
         s with rmState := s.rmState.insert rm RMState.Aborted,
     } else none
 
 /-- Resource manager `rm` is told by the TM to commit. -/
-def rmRcvCommitMsg (rm: RM) :=
+def rmRcvCommitMsg (rm: RM N) :=
     if Message.Commit ∈ s.msgs then some {
         s with rmState := s.rmState.insert rm RMState.Committed,
     } else none
 
 /-- Resource manager `rm` is told by the TM to abort. -/
-def rmRcvAbortMsg (rm: RM) :=
+def rmRcvAbortMsg (rm: RM N) :=
     if Message.Abort ∈ s.msgs then some {
         s with rmState := s.rmState.insert rm RMState.Aborted,
     } else none
