twophase/Twophase/System.lean
@@ -1,12 +1,11 @@
 /-
 This is a specification of the system level of the two-phase commit protocol.
 
-Igor Konnov, 2025
+Copyright (c) 2025 Igor Konnov
+Released under MIT license as described in the file LICENSE.
+Authors: Igor Konnov, 2025
 -/
 import Twophase.Functional
-
--- The abstract type of resource managers.
-variable {RM : Type} [DecidableEq RM] [Hashable RM] [Repr RM]
 
 /--
 Since Lean4 is not TLA+, it does not have a built-in syntax for actions.
@@ -14,26 +13,29 @@ Hence, we introduce the type that essentially turns control and data
 non-deterministm into inputs. This trick is usually called a "schedule"
 or "adversary" in the literature.
 -/
-inductive Action where
+inductive Action (N: Nat) where
   | TMCommit
   | TMAbort
-  | TMRcvPrepared(rm: RM)
-  | RMPrepare(rm: RM)
-  | RMChooseToAbort(rm: RM)
-  | RMRcvCommitMsg(rm: RM)
-  | RMRcvAbortMsg(rm: RM)
+  | TMRcvPrepared(rm: RM N)
+  | RMPrepare(rm: RM N)
+  | RMChooseToAbort(rm: RM N)
+  | RMRcvCommitMsg(rm: RM N)
+  | RMRcvAbortMsg(rm: RM N)
   deriving DecidableEq, Repr
 
+section
+-- The number of resource managers.
+variable { N: Nat }
+
 /-- initialize the state of all resource managers to `Working` -/
-def init_rm_state (all: List RM) :=
-  all.foldl
+def init_rm_state :=
+  (List.finRange N).foldl
     (fun m rm => m.insert rm RMState.Working)
     (Std.HashMap.emptyWithCapacity 0)
 
 /-- The initial state of the protocol -/
-def init (all: List RM): ProtocolState RM := {
-    all := all.toFinset,
-    rmState := init_rm_state all,
+def init: ProtocolState N := {
+    rmState := init_rm_state,
     tmState := TMState.Init,
     tmPrepared := ∅,
     msgs := ∅
@@ -41,12 +43,13 @@ def init (all: List RM): ProtocolState RM := {
 
 /-- The transition function (!) of the protocol. Since we provide `next` with
 the action as an argument, `next` is a function, not a relation. -/
-def next s a :=
+def next (s: ProtocolState N) (a: Action N) :=
   match a with
-  | Action.TMCommit => tmCommit RM s
-  | Action.TMAbort => tmAbort _ s
-  | Action.TMRcvPrepared rm => tmRcvPrepared _ s rm
-  | Action.RMPrepare rm => rmPrepare _ s rm
-  | Action.RMChooseToAbort rm => rmChooseToAbort _ s rm
-  | Action.RMRcvCommitMsg rm => rmRcvCommitMsg _ s rm
-  | Action.RMRcvAbortMsg rm => rmRcvAbortMsg _ s rm
+  | Action.TMCommit => tmCommit s
+  | Action.TMAbort => tmAbort s
+  | Action.TMRcvPrepared rm => tmRcvPrepared s rm
+  | Action.RMPrepare rm => rmPrepare s rm
+  | Action.RMChooseToAbort rm => rmChooseToAbort s rm
+  | Action.RMRcvCommitMsg rm => rmRcvCommitMsg s rm
+  | Action.RMRcvAbortMsg rm => rmRcvAbortMsg s rm
+end
