twophase/Twophase.lean
@@ -1,4 +1,9 @@
--- This module serves as the root of the `Twophase` library.
--- Import modules here that should be built as part of the library.
+/-
+The main module of Twophase.
+
+Copyright (c) 2025 Igor Konnov
+Released under MIT license as described in the file LICENSE.
+Authors: Igor Konnov, 2025
+-/
 import Twophase.Functional
 import Twophase.System
